theories/LogicalRelation.v
@@ -48,27 +48,29 @@ Module LR.
   Import Pred.
   Import Pred.notations.
 
+  #[local] Open Scope pred_scope.
+
   Definition RELATION (Θ : ACC) (A : TYPE) : Type :=
     forall w0 w1 (θ01 : Θ w0 w1),
       A w0 -> A w1 -> Pred w1.
 
   Definition RProper {Θ A} {reflΘ : Refl Θ} (R : RELATION Θ A) {w} (a : A w) : Prop :=
-    PValid (R w w refl a a).
+    entails Trueₚ (R w w refl a a).
 
   Definition RPred (Θ : ACC) {instΘ : forall w, Inst (Θ w) (Assignment w)} :
-    RELATION Θ Pred := fun w0 w1 r01 p0 p1 => PIff (Ext p0 r01) p1.
+    RELATION Θ Pred := fun w0 w1 r01 p0 p1 => Ext p0 r01 <->ₚ p1.
 
-  Definition RBox {Θ A} {transΘ : Trans Θ} {instΘ : forall w, Inst (Θ w) (Assignment w)}
-    (R : RELATION Θ A) : RELATION Θ (Box Θ A) :=
+  Definition RBox Θ {transΘ : Trans Θ} {instΘ : forall w, Inst (Θ w) (Assignment w)}
+     {A} (R : RELATION Θ A) : RELATION Θ (Box Θ A) :=
     fun w0 w1 θ01 ba0 ba1 =>
-      (∀ w2 ∶ Const World,
-       ∀ w3 ∶ Const World,
-       ∀ θ02 ∶ Const (Θ w0 w2),
-       ∀ θ13 ∶ Const (Θ w1 w3),
-       ∀ θ23 ∶ Const (Θ w2 w3),
+       ∀ₚ w2 ∶ Const World,
+       ∀ₚ w3 ∶ Const World,
+       ∀ₚ θ02 ∶ Const (Θ w0 w2),
+       ∀ₚ θ13 ∶ Const (Θ w1 w3),
+       ∀ₚ θ23 ∶ Const (Θ w2 w3),
          Acc.wlp θ13
-           (θ01 ⊙ θ13 ≃ θ02 ⊙ θ23 ⇒
-            R w2 w3 θ23 (ba0 w2 θ02) (ba1 w3 θ13)))%P.
+           (θ01 ⊙ θ13 =ₚ θ02 ⊙ θ23 ->ₚ
+            R w2 w3 θ23 (ba0 w2 θ02) (ba1 w3 θ13)).
 
   (*         Θ01          *)
   (*    w0 -------> w1    *)
@@ -79,26 +81,38 @@ Module LR.
   (*    w2 -------> w3    *)
   (*         θ23          *)
 
+  Import SigTNotations.
+
+  Definition RDiamond Θ {transΘ : Trans Θ} {instΘ : forall w, Inst (Θ w) (Assignment w)}
+    {A} (R : RELATION Θ A) : RELATION Θ (Diamond Θ A) :=
+    fun w0 w1 θ01 da0 da1 =>
+      match da0 , da1 with
+      | (w2; (θ02,a2)) , (w3; (θ13,a3)) =>
+          ∃ₚ θ23 ∶ Const (Θ w2 w3),
+          Acc.wp θ13
+            ((θ01 ⊙ θ13) =ₚ (θ02 ⊙ θ23) /\ₚ
+             R w2 w3 θ23 a2 a3)
+      end.
+
   Definition RImpl {Θ A B} (RA : RELATION Θ A) (RB : RELATION Θ B) : RELATION Θ (Impl A B) :=
     fun w0 w1 θ01 f0 f1 =>
-      (∀ a0 ∶ Const (A w0),
-       ∀ a1 ∶ Const (A w1),
-         RA w0 w1 θ01 a0 a1 ⇒
+      (∀ₚ a0 ∶ Const (A w0),
+       ∀ₚ a1 ∶ Const (A w1),
+         RA w0 w1 θ01 a0 a1 ->ₚ
          RB w0 w1 θ01 (f0 a0) (f1 a1))%P.
 
   Definition RTy {Θ} {pers : Persistent Θ Ty} : RELATION Θ Ty :=
     fun w0 w1 θ01 t0 t1 =>
-      PEq (persist _ t0 _ θ01) t1.
+      persist _ t0 _ θ01 =ₚ t1.
 
   Lemma rty_bool {w0 w1} {θ01 : Tri w0 w1} :
-    PValid (RTy θ01 Ty_bool Ty_bool).
+    ⊤ₚ ⊢ₚ RTy θ01 Ty_bool Ty_bool.
   Proof. unfold RTy. now rewrite Tri.persist_bool. Qed.
 
   Lemma rty_func {w0 w1} (θ01 : Tri w0 w1) (t1_0 t2_0 : Ty w0) (t1_1 t2_1 : Ty w1) :
-    PValid
-      (RTy θ01 t1_0 t1_1 ⇒
-       RTy θ01 t2_0 t2_1 ⇒
-       RTy θ01 (Ty_func t1_0 t2_0) (Ty_func t1_1 t2_1)).
+    ⊤ₚ ⊢ₚ (RTy θ01 t1_0 t1_1 ->ₚ
+           RTy θ01 t2_0 t2_1 ->ₚ
+           RTy θ01 (Ty_func t1_0 t2_0) (Ty_func t1_1 t2_1)).
   Proof.
     unfold RTy. rewrite Tri.persist_func.
     rewrite (peq_ty_noconfusion (Ty_func _ _)).
@@ -108,9 +122,50 @@ Module LR.
 
   Definition RValid {Θ A} (R : RELATION Θ A) (a : ⊢ A) : Prop :=
     forall w0 w1 θ01,
-      PValid (R w0 w1 θ01 (a w0) (a w1)).
+      ⊤ₚ ⊢ₚ R w0 w1 θ01 (a w0) (a w1).
 
   Definition RUnit {Θ} : RELATION Θ Unit :=
-    fun _ _ _ _ _ => PTrue.
+    fun _ _ _ _ _ => Trueₚ.
+
+  Section Option.
+
+    Import Prelude.option.
+
+    Definition ROption {Θ A} (R : RELATION Θ A) : RELATION Θ (Option A) :=
+      fun w0 w1 r01 m0 m1 =>
+        match m0 , m1 with
+        | Some a0 , Some a1 => R w0 w1 r01 a0 a1
+        | Some _  , None    => Trueₚ
+        | None    , Some _  => Falseₚ
+        | None    , None    => Trueₚ
+        end.
+
+    Lemma proper_option_bind {Θ} {transR : Trans Θ}
+      {instΘ : forall w, Inst (Θ w) (Assignment w)}
+      {A B} (RA : RELATION Θ A) (RB : RELATION Θ B) :
+      RValid
+        (RImpl (ROption RA) (RImpl (RImpl RA (ROption RB)) (ROption RB)))
+        (fun w => bind).
+    Proof.
+      intros w0 w1 r01.
+      apply forall_r. intros m0.
+      apply forall_r. intros m1.
+      apply impl_and_adjoint. rewrite and_true_l.
+      apply forall_r. intros f0.
+      apply forall_r. intros f1.
+      apply impl_and_adjoint.
+      (* cbv [Entails ROption RImpl ROption PImpl Forall Const Impl Option] in *. *)
+      (* intros ι [rm rf]. *)
+      destruct m0 as [a0|], m1 as [a1|]; cbn.
+      - rewrite and_comm. apply impl_and_adjoint.
+        apply forall_l. exists a0.
+        apply forall_l. exists a1.
+        reflexivity.
+      - now destruct (f0 a0).
+      - rewrite and_false_l. easy.
+      - easy.
+    Qed.
+
+  End Option.
 
 End LR.
