theories/Predicates.v
@@ -46,6 +46,8 @@ Set Implicit Arguments.
 
 Module Pred.
 
+  #[local] Notation Expr := (Sem expr).
+
   Declare Scope pred_scope.
   Delimit Scope pred_scope with P.
 
@@ -53,232 +55,299 @@ Module Pred.
     Assignment w -> Prop.
   Bind Scope pred_scope with Pred.
 
-  Section Connectives.
+  Section RewriteRelations.
 
     Context {w : World}.
 
-    Definition PValid {w} (P : Pred w) : Prop :=
-      forall ι, P ι.
-    Definition PUnsatisfiable {w} (P : Pred w) : Prop :=
-      forall ι, ~ P ι.
-
-    Definition BiEntails : relation (Pred w) :=
+    Definition bientails : relation (Pred w) :=
       fun P Q => forall ι, P ι <-> Q ι.
-    Definition Entails : relation (Pred w) :=
+    Definition entails : relation (Pred w) :=
       fun P Q => forall ι, P ι -> Q ι.
 
-    #[export] Instance equivalence_bientails : Equivalence BiEntails.
+    #[export] Instance equivalence_bientails : Equivalence bientails.
     Proof.
-      constructor; unfold Reflexive, Symmetric, Transitive, BiEntails;
+      constructor; unfold Reflexive, Symmetric, Transitive, bientails;
         [ reflexivity | now symmetry | now etransitivity ].
     Qed.
-    #[export] Instance preorder_entails : RelationClasses.PreOrder Entails.
-    Proof. constructor; unfold Reflexive, Transitive, Entails; auto. Qed.
+    #[export] Instance preorder_entails : RelationClasses.PreOrder entails.
+    Proof. constructor; unfold Reflexive, Transitive, entails; auto. Qed.
 
     #[export] Instance subrelation_bientails_entails :
-      subrelation BiEntails Entails.
+      subrelation bientails entails.
     Proof. intros x y xy ι. apply xy. Qed.
 
     #[export] Instance subrelation_bientails_flip_entails :
-      subrelation BiEntails (Basics.flip Entails).
+      subrelation bientails (Basics.flip entails).
     Proof. intros x y xy ι. apply xy. Qed.
 
     (* #[export] Instance proper_bientails : *)
-    (*   Proper (BiEntails ==> BiEntails ==> iff) BiEntails. *)
+    (*   Proper (bientails ==> bientails ==> iff) bientails. *)
     (* Proof. intuition. Qed. *)
     #[export] Instance proper_entails_bientails :
-      Proper (BiEntails ==> BiEntails ==> iff) Entails.
-    Proof. unfold Proper, respectful, BiEntails, Entails. intuition. Qed.
+      Proper (bientails ==> bientails ==> iff) entails.
+    Proof. unfold Proper, respectful, bientails, entails. intuition. Qed.
     #[export] Instance proper_entails_entails :
-      Proper (Basics.flip Entails ==> Entails ==> Basics.impl) Entails.
-    Proof. unfold Proper, respectful, Basics.impl, Entails. intuition. Qed.
+      Proper (Basics.flip entails ==> entails ==> Basics.impl) entails.
+    Proof. unfold Proper, respectful, Basics.impl, entails. intuition. Qed.
 
-    Definition PFalse : Pred w :=
-      fun _ => False.
-    Definition PTrue : Pred w :=
-      fun _ => True.
-    Definition PIff (P Q : Pred w) : Pred w :=
-      fun ι => P ι <-> Q ι.
-    Definition PImpl (P Q : Pred w) : Pred w :=
-      fun ι => (P ι -> Q ι)%type.
-    Definition PAnd (P Q : Pred w) : Pred w :=
-      fun ι => (P ι /\ Q ι)%type.
+  End RewriteRelations.
+  #[global] Arguments bientails {w} (_ _)%P.
+  #[global] Arguments entails {w} (_ _)%P.
+  #[global] Typeclasses Opaque entails.
+  #[global] Typeclasses Opaque bientails.
 
-    #[export] Instance proper_pvalid_bientails : Proper (BiEntails ==> iff) PValid.
-    Proof. firstorder. Qed.
-    #[export] Instance proper_pvalid_entails : Proper (Entails ==> Basics.impl) PValid.
-    Proof. firstorder. Qed.
-    #[export] Instance proper_piff : Proper (BiEntails ==> BiEntails ==> BiEntails) PIff.
-    Proof. firstorder. Qed.
-    #[export] Instance proper_pimpl_bientails : Proper (BiEntails ==> BiEntails ==> BiEntails) PImpl.
-    Proof. firstorder. Qed.
-    #[export] Instance proper_pimpl_entails : Proper (Entails --> Entails ==> Entails) PImpl.
-    Proof. firstorder. Qed.
-    #[export] Instance proper_pand_bientails : Proper (BiEntails ==> BiEntails ==> BiEntails) PAnd.
-    Proof. firstorder. Qed.
-    #[export] Instance proper_pand_entails : Proper (Entails ==> Entails ==> Entails) PAnd.
-    Proof. firstorder. Qed.
+  Section Definitions.
 
-  End Connectives.
-  #[global] Arguments BiEntails {w} (_ _)%P.
-  #[global] Arguments Entails {w} (_ _)%P.
-  #[global] Arguments PAnd {_} _ _ _/.
-  #[global] Arguments PImpl {_} _ _ _/.
-  #[global] Arguments PFalse {_} _/.
+    Definition Falseₚ : ⊢ Pred :=
+      fun w _ => Logic.False.
+    Definition Trueₚ : ⊢ Pred :=
+      fun w _ => Logic.True.
+    Definition iffₚ : ⊢ Pred -> Pred -> Pred :=
+      fun w P Q ι => P ι <-> Q ι.
+    Definition implₚ : ⊢ Pred -> Pred -> Pred :=
+      fun w P Q ι => (P ι -> Q ι)%type.
+    Definition andₚ : ⊢ Pred -> Pred -> Pred :=
+      fun w P Q ι => (P ι /\ Q ι)%type.
+    #[global] Arguments andₚ {_} (_ _)%P _/.
+    #[global] Arguments iffₚ {_} (_ _)%P _/.
+    #[global] Arguments implₚ {_} (_ _)%P _/.
+    #[global] Arguments Trueₚ {_} _/.
+    #[global] Arguments Falseₚ {_} _/.
 
-  Definition Forall {I : TYPE} : ⊢ (I -> Pred) -> Pred :=
-    fun w A ι => forall i : I w, A i ι.
-  Definition Exists {I : TYPE} : ⊢ (I -> Pred) -> Pred :=
-    fun w A ι => exists i : I w, A i ι.
-  #[global] Arguments Forall {I w} A ι.
-  #[global] Arguments Exists {I w} A ι.
-
-  #[local] Notation "⊩ P" := (PValid P) (at level 95).
-  #[local] Notation "P ⊣⊢ Q" := (BiEntails P Q) (at level 95).
-  #[local] Notation "⊤" := PTrue : pred_scope.
-  #[local] Notation "⊥" := PFalse : pred_scope.
-  #[local] Notation "P ⇔ Q" := (PIff P Q) (at level 94) : pred_scope.
-  #[local] Notation "P ⇒ Q" := (PImpl P Q) (at level 94, right associativity) : pred_scope.
-  #[local] Notation "P ∧ Q" := (PAnd P Q) (at level 80, right associativity) : pred_scope.
-
-  Lemma pimpl_and_adjoint {w} (P Q R : Pred w) :
-    Entails (P ∧ Q) R <-> Entails P (Q ⇒ R).
-  Proof. unfold Entails, PAnd, PImpl. intuition. Qed.
-
-  Lemma split_bientails {w} (P Q : Pred w) :
-    BiEntails P Q <-> Entails P Q /\ Entails Q P.
-  Proof. unfold Entails, BiEntails. firstorder. Qed.
-
-  Lemma pand_comm {w} (P Q : Pred w) : P ∧ Q ⊣⊢ Q ∧ P.
-  Proof. unfold BiEntails, PAnd. intuition. Qed.
-  Lemma pand_true_l {w} (P : Pred w) : ⊤ ∧ P ⊣⊢ P.
-  Proof. now unfold BiEntails, PAnd, PTrue. Qed.
-  Lemma pand_true_r {w} (P : Pred w) : P ∧ ⊤ ⊣⊢ P.
-  Proof. now unfold BiEntails, PAnd, PTrue. Qed.
-  Lemma pand_false_l {w} (P : Pred w) : PFalse ∧ P ⊣⊢ PFalse.
-  Proof. now unfold BiEntails, PAnd, PFalse. Qed.
-  Lemma pand_false_r {w} (P : Pred w) : P ∧ PFalse ⊣⊢ PFalse.
-  Proof. now unfold BiEntails, PAnd, PFalse. Qed.
-  Lemma pimpl_true_l {w} (P : Pred w) : ⊤ ⇒ P ⊣⊢ P.
-  Proof. unfold BiEntails, PImpl, PTrue. intuition. Qed.
-  Lemma pimpl_true_r {w} (P : Pred w) : P ⇒ ⊤ ⊣⊢ ⊤.
-  Proof. unfold BiEntails, PImpl, PTrue. intuition. Qed.
-  Lemma pimpl_false_l {w} (P : Pred w) : ⊥ ⇒ P ⊣⊢ ⊤.
-  Proof. unfold BiEntails, PImpl, PTrue, PFalse. intuition. Qed.
-  Lemma entails_false {w} (P : Pred w) : Entails PFalse P.
-  Proof. easy. Qed.
-  Lemma entails_true {w} (P : Pred w) : Entails P PTrue.
-  Proof. easy. Qed.
-
-  Lemma pPoseProof {w} {P Q R : Pred w} :
-    PValid Q -> Entails (P ∧ Q) R -> Entails P R.
-  Proof. unfold PValid, Entails, PAnd. intuition. Qed.
-
-  Lemma pGeneralize {w} {P Q R : Pred w} :
-    PValid Q -> Entails P (Q ⇒ R) -> Entails P R.
-  Proof. unfold PValid, Entails, PAnd. intuition. Qed.
-
-  Lemma pApply {w} {P Q R : Pred w} :
-    Entails P Q -> Entails Q R -> Entails P R.
-  Proof. apply transitivity. Qed.
-
-  Lemma pApply_r {w} {P Q R : Pred w} :
-    Entails Q R -> Entails P Q -> Entails P R.
-  Proof. intros; etransitivity; eauto. Qed.
-
-  Lemma pIntro {w} {P Q : Pred w} :
-    Entails P Q -> PValid (P ⇒ Q).
-  Proof. now unfold PValid, Entails, PImpl. Qed.
-
-  Section Ext.
-
-    Context {R : ACC} {instR : forall w, Inst (R w) (Assignment w)}.
-
-    Definition Ext  : ⊢ Pred -> Box R Pred :=
-      fun w0 p w1 r ι => p (inst r ι).
-    #[global] Arguments Ext [w] _%P [w1].
-
-    #[export] Instance proper_ext_bientails {w : World} :
-      Proper (BiEntails ==> forall_relation (fun _ => eq ==> BiEntails)) (@Ext w).
-    Proof. intros p q pq w1 ? ? ? ι; subst; apply pq. Qed.
-    #[export] Instance proper_ext_entails {w : World} :
-      Proper (Entails ==> forall_relation (fun _ => eq ==> Entails)) (@Ext w).
-    Proof. intros p q pq w1 ? ? ? ι; subst; apply pq. Qed.
-
-    Lemma ext_refl {reflR : Refl R} {instReflR : InstRefl R} {w} (P : Pred w) :
-      BiEntails (Ext P refl) P.
-    Proof. unfold BiEntails, Ext. intros ι. now rewrite inst_refl. Qed.
-
-    Lemma ext_trans {transR : Trans R} {w0 w1 w2} (r1 : R w0 w1) (r2 : R w1 w2)
-      (P : Pred w0) :
-      BiEntails (Ext P (trans r1 r2)) (Ext (Ext P r1) r2).
-    Proof. unfold BiEntails, Ext. intros ι. now rewrite inst_trans. Qed.
-
-    Lemma ext_and {w0 w1} (ζ01 : R w0 w1) (P Q : Pred w0) :
-      Ext P ζ01 ∧ Ext Q ζ01 ⊣⊢ Ext (P ∧ Q) ζ01 .
-    Proof. unfold BiEntails, Ext, PAnd. intuition. Qed.
-
-    Lemma ext_impl {w0 w1} (ζ01 : R w0 w1) (P Q : Pred w0) :
-      Ext P ζ01 ⇒ Ext Q ζ01 ⊣⊢ Ext (P ⇒ Q) ζ01 .
-    Proof. unfold BiEntails, Ext, PAnd. intuition. Qed.
-
-    Lemma ext_false {w0 w1} (ζ01 : R w0 w1) :
-      Ext PFalse ζ01 ⊣⊢ PFalse.
-    Proof. unfold BiEntails, Ext, PFalse. reflexivity. Qed.
-
-    Lemma ext_true {w0 w1} (ζ01 : R w0 w1) :
-      Ext PTrue ζ01 ⊣⊢ PTrue.
-    Proof. unfold BiEntails, Ext, PTrue. reflexivity. Qed.
-
-  End Ext.
-  #[global] Arguments Ext {_ _} [w] _ [_] _ _/.
-  #[global] Instance params_ext : Params (@Ext) 6 := {}.
-
-  Section Eq.
-
-    Context {T : TYPE} {A : Type} {instTA : Inst T A}.
-
-    Definition PEq : ⊢ T -> T -> Pred :=
+    Definition eqₚ {T : TYPE} {A : Type} {instTA : Inst T A} :
+      ⊢ T -> T -> Pred :=
       fun w t1 t2 ι => inst t1 ι = inst t2 ι.
-    #[local] Infix "=" := PEq : pred_scope.
+    #[global] Arguments eqₚ {T A _} [w] _ _ _/.
 
-    Lemma peq_refl {w} (t : T w) :
-      PEq t t ⊣⊢ ⊤.
-    Proof. easy. Qed.
+    Definition Forall {I : TYPE} : ⊢ (I -> Pred) -> Pred :=
+      fun w A ι => forall i : I w, A i ι.
+    Definition Exists {I : TYPE} : ⊢ (I -> Pred) -> Pred :=
+      fun w A ι => exists i : I w, A i ι.
+    #[global] Arguments Forall {I w} A%P ι/.
+    #[global] Arguments Exists {I w} A%P ι/.
 
-    Lemma peq_symmetry {w} (s t : T w) :
-      PEq s t ⊣⊢ PEq t s.
-    Proof. easy. Qed.
+    Definition Ext {R : ACC} {instR : forall w, Inst (R w) (Assignment w)} :
+      ⊢ Pred -> Box R Pred :=
+      fun w0 p w1 r ι => p (inst r ι).
+    #[global] Arguments Ext {_ _} [w] _%P [_] _ _/.
+    #[global] Instance params_ext : Params (@Ext) 6 := {}.
 
-    Lemma peq_persist {R : ACC} {persR : Persistent R T}
-      (instR : forall w : World, Inst (R w) (Assignment w))
-      {w0 w1} (r : R w0 w1) (t1 t2 : T w0) :
-      PEq (persist _ t1 _ r) (persist _ t2 _ r) ⊣⊢ Ext (PEq t1 t2) r.
-    Proof.
-      unfold BiEntails, PEq, Ext. intros ι.
-      (* now rewrite !inst_persist. *)
-    Admitted.
+    Definition TPB : ⊢ Env -> Const expr -> Ty -> Expr -> Pred :=
+      fun w G e t ee ι => inst G ι |-- e ; inst t ι ~> inst ee ι.
+    #[global] Arguments TPB [w] G e t ee ι/.
 
-  End Eq.
-  #[global] Arguments PEq {T A _} [w] _ _ _/.
-  #[local] Infix "=" := PEq : pred_scope.
+  End Definitions.
 
-  Lemma peq_ty_noconfusion {w} (t1 t2 : Ty w) :
-    t1 = t2 ⊣⊢
-      match t1 , t2 with
-      | Ty_bool         , Ty_bool         => PTrue
-      | Ty_func t11 t12 , Ty_func t21 t22 => PEq t11 t21 ∧ PEq t12 t22
-      | Ty_hole _       , _               => PEq t1 t2
-      | _               , Ty_hole _       => PEq t1 t2
-      | _               , _               => PFalse
-      end.
-  Proof.
-    intros ι; unfold PEq, PFalse, PTrue, PAnd; destruct t1, t2;
-      cbn; try reflexivity; intuition congruence.
-  Qed.
+  Module Import notations.
 
-  #[global] Typeclasses Opaque Entails.
-  #[global] Typeclasses Opaque BiEntails.
+    Infix "⊣⊢ₚ" := (bientails) (at level 95).
+    Infix "⊢ₚ" := (entails) (at level 95).
+
+    Notation "⊤ₚ" := Trueₚ : pred_scope.
+    Notation "⊥ₚ" := Falseₚ : pred_scope.
+    Infix "<->ₚ"  := (iffₚ) (at level 94) : pred_scope.
+    Infix "->ₚ"   := (implₚ) (at level 94, right associativity) : pred_scope.
+    Infix "/\ₚ"   := (andₚ) (at level 80, right associativity) : pred_scope.
+
+    Infix "=ₚ" := eqₚ (at level 70, no associativity) : pred_scope.
+
+    Notation "'∀ₚ' x ∶ T , Q" :=
+      (@Forall T _ (fun x => Q%P))
+        (at level 99, x binder, x at next level, T at level 95,
+          right associativity,
+          format "'∀ₚ'  x  ∶  T ,  Q")
+      : pred_scope.
+
+    Notation "'∀ₚ⁺' x .. y , Q " :=
+      (Forall (fun x => .. (Forall (fun y => Q%P)) ..))
+        (at level 99, x binder, y binder, right associativity,
+        only parsing)
+      : pred_scope.
+
+    (* Notation "'∃' x .. y , Q " := *)
+    (*     (Exists (fun x => .. (Exists (fun y => Q%P)) ..)) *)
+    (*       (at level 94, x binder, y binder, right associativity) *)
+    (*     : pred_scope. *)
+
+    Notation "'∃ₚ' x ∶ T , Q" :=
+      (@Exists T _ (fun x => Q%P))
+        (at level 99, x binder, right associativity,
+          format "'∃ₚ'  x  ∶  T ,  Q")
+        : pred_scope.
+
+    Notation "'Fun' x => b" :=
+      (fun w ζ x => b%P w ζ)
+        (x binder, at level 100) : pred_scope.
+
+    Notation "G |--ₚ E ; T ~> EE" :=
+      (TPB G E T EE) (at level 70, no associativity) : pred_scope.
+
+  End notations.
+
+  Section Lemmas.
+
+    Create HintDb obligation.
+    #[local] Hint Rewrite @inst_refl @inst_trans : obligation.
+
+    #[local] Ltac obligation :=
+      unfold Proper, respectful, pointwise_relation, forall_relation,
+        entails, bientails;
+        cbn; intros; subst;
+      try (match goal with
+         | |- (forall _ : ?A, _) <-> (forall _ : ?A, _) =>
+             apply all_iff_morphism; intro
+         | |- (exists _ : ?A, _) <-> (exists _ : ?A, _) =>
+             apply ex_iff_morphism; intro
+         end);
+      autorewrite with obligation;
+      try easy; try (intuition; fail); try (intuition congruence; fail).
+    #[local] Obligation Tactic := obligation.
+
+    #[export,program] Instance proper_iff {w} :
+      Proper (bientails ==> bientails ==> bientails) (@iffₚ w).
+    #[export,program] Instance proper_impl_bientails {w} :
+      Proper (bientails ==> bientails ==> bientails) (@implₚ w).
+    #[export,program] Instance proper_impl_entails {w} :
+      Proper (entails --> entails ==> entails) (@implₚ w).
+    #[export,program] Instance proper_and_bientails {w} :
+      Proper (bientails ==> bientails ==> bientails) (@andₚ w).
+    #[export,program] Instance proper_and_entails {w} :
+      Proper (entails ==> entails ==> entails) (@andₚ w).
+    #[export,program] Instance proper_bientails_forall {I w} :
+      Proper (pointwise_relation (I w) bientails ==> bientails) Forall.
+    #[export,program] Instance proper_bientails_exists {I w} :
+      Proper (pointwise_relation (I w) bientails ==> bientails) Exists.
+    #[export,program] Instance proper_ext_bientails
+      {R : ACC} {instR : forall w, Inst (R w) (Assignment w)} {w} :
+      Proper (bientails ==> forall_relation (fun _ => eq ==> bientails)) (Ext (R:=R) (w:=w)).
+    #[export,program] Instance proper_ext_entails
+      {R : ACC} {instR : forall w, Inst (R w) (Assignment w)} {w} :
+      Proper (entails ==> forall_relation (fun _ => eq ==> entails)) (Ext (R:=R) (w:=w)).
+
+    Lemma split_bientails {w} (P Q : Pred w) :
+      (P ⊣⊢ₚ Q) <-> (P ⊢ₚ Q) /\ (Q ⊢ₚ P).
+    Proof. obligation. Qed.
+    Lemma and_left1 {w} {P Q R : Pred w} : P ⊢ₚ R -> P /\ₚ Q ⊢ₚ R.
+    Proof. obligation. Qed.
+    Lemma and_left2 {w} {P Q R : Pred w} : Q ⊢ₚ R -> P /\ₚ Q ⊢ₚ R.
+    Proof. obligation. Qed.
+    Lemma and_right {w} {P Q R : Pred w} : P ⊢ₚ Q -> P ⊢ₚ R -> P ⊢ₚ Q /\ₚ R.
+    Proof. obligation. Qed.
+    Lemma impl_and_adjoint {w} (P Q R : Pred w) : (P /\ₚ Q ⊢ₚ R) <-> (P ⊢ₚ Q ->ₚ R).
+    Proof. obligation. Qed.
+    Lemma and_comm {w} (P Q : Pred w) : P /\ₚ Q  ⊣⊢ₚ  Q /\ₚ P.
+    Proof. obligation. Qed.
+    Lemma and_assoc {w} (P Q R : Pred w) : (P /\ₚ Q) /\ₚ R  ⊣⊢ₚ  P /\ₚ (Q /\ₚ R).
+    Proof. obligation. Qed.
+    Lemma and_true_l {w} (P : Pred w) : ⊤ₚ /\ₚ P ⊣⊢ₚ P.
+    Proof. obligation. Qed.
+    Lemma and_true_r {w} (P : Pred w) : P /\ₚ ⊤ₚ ⊣⊢ₚ P.
+    Proof. obligation. Qed.
+    Lemma and_false_l {w} (P : Pred w) : ⊥ₚ /\ₚ P ⊣⊢ₚ ⊥ₚ.
+    Proof. obligation. Qed.
+    Lemma and_false_r {w} (P : Pred w) : P /\ₚ ⊥ₚ ⊣⊢ₚ ⊥ₚ.
+    Proof. obligation. Qed.
+    Lemma impl_true_l {w} (P : Pred w) : ⊤ₚ ->ₚ P ⊣⊢ₚ P.
+    Proof. obligation. Qed.
+    Lemma impl_true_r {w} (P : Pred w) : P ->ₚ ⊤ₚ ⊣⊢ₚ ⊤ₚ.
+    Proof. obligation. Qed.
+    Lemma impl_false_l {w} (P : Pred w) : ⊥ₚ ->ₚ P ⊣⊢ₚ ⊤ₚ.
+    Proof. obligation. Qed.
+    Lemma false_l {w} (P : Pred w) : ⊥ₚ ⊢ₚ P.
+    Proof. obligation. Qed.
+    Lemma true_r {w} (P : Pred w) : P ⊢ₚ ⊤ₚ.
+    Proof. obligation. Qed.
+
+    Lemma forall_l {I : TYPE} {w} (P : I w -> Pred w) Q :
+      (exists x : I w, P x ⊢ₚ Q) -> (∀ₚ x ∶ I, P x) ⊢ₚ Q.
+    Proof. obligation. firstorder. Qed.
+    Lemma forall_r {I : TYPE} {w} P (Q : I w -> Pred w) :
+      (P ⊢ₚ (∀ₚ x ∶ I, Q x)) <-> (forall x : I w, P ⊢ₚ Q x).
+    Proof. obligation. Qed.
+
+    Lemma exists_l {I : TYPE} {w} P (Q : I w -> Pred w) :
+      (exists x : I w, P ⊢ₚ Q x) -> P ⊢ₚ (∃ₚ x ∶ I, Q x).
+    Proof. obligation. firstorder. Qed.
+    Lemma exists_r {I : TYPE} {w} P (Q : I w -> Pred w) :
+      (exists x : I w, P ⊢ₚ Q x) -> P ⊢ₚ (∃ₚ x ∶ I, Q x).
+    Proof. obligation. firstorder. Qed.
+    #[global] Arguments exists_r {I w P Q} _.
+
+    Lemma pApply {w} {P Q R : Pred w} :
+      P ⊢ₚ Q -> Q ⊢ₚ R -> P ⊢ₚ R.
+    Proof. now transitivity Q. Qed.
+
+    Lemma pApply_r {w} {P Q R : Pred w} :
+      Q ⊢ₚ R -> P ⊢ₚ Q -> P ⊢ₚ R.
+    Proof. now transitivity Q. Qed.
+
+    Section Eq.
+
+      Context {T A} {instTA : Inst T A}.
+
+      Lemma eqₚ_refl {w} (t : T w) : t =ₚ t ⊣⊢ₚ ⊤ₚ.
+      Proof. obligation. Qed.
+
+      Lemma eqₚ_symmetry {w} (s t : T w) : s =ₚ t ⊣⊢ₚ t =ₚ s.
+      Proof. obligation. Qed.
+
+    End Eq.
+
+    Lemma peq_ty_noconfusion {w} (t1 t2 : Ty w) :
+      t1 =ₚ t2 ⊣⊢ₚ
+            match t1 , t2 with
+            | Ty_bool         , Ty_bool         => ⊤ₚ
+            | Ty_func t11 t12 , Ty_func t21 t22 => t11 =ₚ t21 /\ₚ t12 =ₚ t22
+            | Ty_hole _       , _               => t1 =ₚ t2
+            | _               , Ty_hole _       => t1 =ₚ t2
+            | _               , _               => ⊥ₚ
+            end.
+    Proof. destruct t1, t2; obligation. Qed.
+
+    Section Ext.
+
+      Context {R : ACC} {instR : forall w, Inst (R w) (Assignment w)}.
+
+      Lemma ext_refl {reflR : Refl R} {instReflR : InstRefl R} {w} (P : Pred w) :
+        Ext P refl ⊣⊢ₚ P.
+      Proof. obligation. Qed.
+      Lemma ext_trans {transR : Trans R}
+        {w0 w1 w2} (r1 : R w0 w1) (r2 : R w1 w2) (P : Pred w0) :
+        Ext P (r1 ⊙ r2) ⊣⊢ₚ Ext (Ext P r1) r2.
+      Proof. obligation. Qed.
+      Lemma ext_and {w0 w1} (ζ01 : R w0 w1) (P Q : Pred w0) :
+        Ext (P /\ₚ Q) ζ01 ⊣⊢ₚ Ext P ζ01 /\ₚ Ext Q ζ01.
+      Proof. obligation. Qed.
+      Lemma ext_impl {w0 w1} (ζ01 : R w0 w1) (P Q : Pred w0) :
+        Ext (P ->ₚ Q) ζ01 ⊣⊢ₚ (Ext P ζ01 ->ₚ Ext Q ζ01).
+      Proof. obligation. Qed.
+      Lemma ext_false {w0 w1} (ζ01 : R w0 w1) :
+        Ext ⊥ₚ ζ01 ⊣⊢ₚ ⊥ₚ.
+      Proof. obligation. Qed.
+      Lemma ext_true {w0 w1} (ζ01 : R w0 w1) :
+        Ext ⊤ₚ ζ01 ⊣⊢ₚ ⊤ₚ.
+      Proof. obligation. Qed.
+      Lemma ext_eq {T : TYPE} {persR : Persistent R T}
+        {A : Type} {instTA : Inst T A}
+        {w0 w1} (r : R w0 w1) (t1 t2 : T w0) :
+        Ext (t1 =ₚ t2) r ⊣⊢ₚ persist w0 t1 w1 r =ₚ persist w0 t2 w1 r.
+      Proof.
+        unfold bientails, eqₚ, Ext. intros ι.
+        (* now rewrite !inst_persist. *)
+      Admitted.
+
+      Lemma ext_forall_const {A} {w1 w2} (r12 : R w1 w2) (Q : A -> Pred w1) :
+        Ext (∀ₚ a ∶ Const A, Q a) r12 ⊣⊢ₚ (∀ₚ a ∶ Const A, Ext (Q a) r12).
+      Proof. obligation. Qed.
+      Lemma ext_tpb {persRTy : Persistent R Ty}
+        {w1 w2} (r12 : R w1 w2) G (e : expr) (t : Ty w1) (ee : Expr w1) :
+        Ext (G |--ₚ e; t ~> ee) r12 ⊣⊢ₚ
+        persist w1 G w2 r12 |--ₚ persist w1 e w2 r12; persist w1 t w2 r12 ~> persist w1 ee w2 r12.
+      Proof. obligation. now rewrite inst_persist_ty, inst_persist_env. Qed.
+
+    End Ext.
+
+  End Lemmas.
 
   (* A type class for things that can be interpreted as a predicate. *)
   Class InstPred (A : TYPE) :=
@@ -286,14 +355,14 @@ Module Pred.
 
   #[export] Instance instpred_option {A} `{ipA : InstPred A} :
     InstPred (Option A) :=
-    fun w o => match o with Some p => instpred p | None => PFalse end.
+    fun w o => match o with Some p => instpred p | None => Falseₚ end.
   #[export] Instance instpred_list {A} `{ipA : InstPred A} :
     InstPred (List A) :=
     fun w =>
       fix ip xs {struct xs} :=
       match xs with
-      | nil       => PTrue
-      | cons y ys => PAnd (instpred y) (ip ys)
+      | nil       => Trueₚ
+      | cons y ys => andₚ (instpred y) (ip ys)
       end.
 
   Module Acc.
@@ -310,32 +379,32 @@ Module Pred.
       #[local] Arguments wlp {_ _} _ _ _/.
 
       #[export] Instance proper_wp_bientails {w0 w1} (r01 : R w0 w1) :
-        Proper (BiEntails ==> BiEntails) (@wp w0 w1 r01).
+        Proper (bientails ==> bientails) (@wp w0 w1 r01).
       Proof.
         intros p q pq ι. cbn. apply ex_iff_morphism.
         intros ι1. apply and_iff_morphism. easy. apply pq.
       Qed.
 
       #[export] Instance proper_wp_entails {w0 w1} (r01 : R w0 w1) :
-        Proper (Entails ==> Entails) (@wp w0 w1 r01).
+        Proper (entails ==> entails) (@wp w0 w1 r01).
       Proof.
         intros p q pq ι. cbn. intros (ι0 & Heq & HP).
         exists ι0. split. easy. now apply pq.
       Qed.
 
       #[export] Instance proper_wlp_bientails {w0 w1} (r01 : R w0 w1) :
-        Proper (BiEntails ==> BiEntails) (@wlp w0 w1 r01).
+        Proper (bientails ==> bientails) (@wlp w0 w1 r01).
       Proof.
         intros p q pq ι. cbn. apply all_iff_morphism. intros ι1.
         now apply iff_iff_iff_impl_morphism.
       Qed.
 
       #[export] Instance proper_wlp_entails {w0 w1} (r01 : R w0 w1) :
-        Proper (Entails ==> Entails) (@wlp w0 w1 r01).
+        Proper (entails ==> entails) (@wlp w0 w1 r01).
       Proof. intros P Q HPQ ι HP ι0 Heq. now apply HPQ, HP. Qed.
 
       Lemma wp_refl {reflR : Refl R} {instReflR : InstRefl R}
-        {w} (Q : Pred w) : wp refl Q ⊣⊢ Q.
+        {w} (Q : Pred w) : wp refl Q ⊣⊢ₚ Q.
       Proof.
         split; cbn.
         - intros (ι' & Heq & HQ). rewrite inst_refl in Heq. now subst.
@@ -344,7 +413,7 @@ Module Pred.
 
       Lemma wp_trans {transR : Trans R}
         {w0 w1 w2} (r01 : R w0 w1) (r12 : R w1 w2) Q :
-        wp (r01 ⊙ r12) Q ⊣⊢ wp r01 (wp r12 Q).
+        wp (r01 ⊙ r12) Q ⊣⊢ₚ wp r01 (wp r12 Q).
       Proof.
         split; cbn.
         - intros (ι2 & Heq & HQ). rewrite inst_trans in Heq.
@@ -354,11 +423,26 @@ Module Pred.
       Qed.
 
       Lemma wp_false {w0 w1} (r01 : R w0 w1) :
-        wp r01 PFalse ⊣⊢ PFalse.
+        wp r01 ⊥ₚ ⊣⊢ₚ ⊥ₚ.
       Proof. firstorder. Qed.
 
+      Lemma wp_step {stepR : Step R} {w} {x} (Q : Pred (ctx.snoc w x)):
+        wp (w0:=w) step Q ⊣⊢ₚ (∃ₚ t ∶ Ty, Ext Q (thick (xIn := ctx.in_zero) x t)).
+      Proof.
+        intros ι. cbn - [thick]. unfold Exists.
+        split.
+        - intros (ι' & <- & HQ). destruct (env.view ι') as [ι t].
+          rewrite inst_step_snoc. exists (lift t _). cbn - [thick].
+          rewrite (inst_thick ctx.in_zero (lift t w) ι).
+          now rewrite inst_lift.
+        - cbn - [thick]. intros (t & HQ).
+          exists (env.snoc ι _ (inst t ι)).
+          rewrite inst_step_snoc.
+          now rewrite (inst_thick ctx.in_zero t ι) in HQ.
+      Qed.
+
       Lemma and_wp_l {w0 w1} (r01 : R w0 w1) P Q :
-        wp r01 P ∧ Q ⊣⊢ wp r01 (P ∧ Ext Q r01).
+        wp r01 P /\ₚ Q ⊣⊢ₚ wp r01 (P /\ₚ Ext Q r01).
       Proof.
         split; cbn.
         - intros [(ι1 & <- & HP) HQ]. now exists ι1.
@@ -366,12 +450,12 @@ Module Pred.
       Qed.
 
       Lemma and_wp_r {w0 w1} (r01 : R w0 w1) P Q :
-        P ∧ wp r01 Q ⊣⊢ wp r01 (Ext P r01 ∧ Q).
-      Proof. now rewrite pand_comm, and_wp_l, pand_comm. Qed.
+        P /\ₚ wp r01 Q ⊣⊢ₚ wp r01 (Ext P r01 /\ₚ Q).
+      Proof. now rewrite and_comm, and_wp_l, and_comm. Qed.
 
       Lemma wp_thick {thickR : Thick R} {instThickR : InstThick R}
-        {w x} (xIn : ctx.In x w) (t : Ty (ctx.remove xIn)) (Q : Pred (ctx.remove xIn))  :
-        wp (thick x t) Q ⊣⊢ PEq (Ty_hole xIn) (thin xIn t) ∧ Ext Q (Sub.thin xIn).
+        {w x} (xIn : ctx.In x w) (t : Ty (ctx.remove xIn)) (Q : Pred (ctx.remove xIn)) :
+        wp (thick x t) Q ⊣⊢ₚ Ty_hole xIn =ₚ thin xIn t /\ₚ Ext Q (Sub.thin xIn).
       Proof.
         intros ι; cbn. rewrite Sub.subst_thin, inst_persist_ty, Sub.inst_thin.
         split.
@@ -382,7 +466,7 @@ Module Pred.
       Qed.
 
       Lemma wlp_refl {reflR : Refl R} {instReflR : InstRefl R}
-        {w} (Q : Pred w) : wlp refl Q ⊣⊢ Q.
+        {w} (Q : Pred w) : wlp refl Q ⊣⊢ₚ Q.
       Proof.
         split; cbn.
         - intros HQ. apply HQ. now rewrite inst_refl.
@@ -391,7 +475,7 @@ Module Pred.
 
       Lemma wlp_trans {transR : Trans R}
         {w0 w1 w2} (r01 : R w0 w1) (r12 : R w1 w2) Q :
-        wlp (r01 ⊙ r12) Q ⊣⊢ wlp r01 (wlp r12 Q).
+        wlp (r01 ⊙ r12) Q ⊣⊢ₚ wlp r01 (wlp r12 Q).
       Proof.
         split; cbn.
         - intros HQ ι1 Heq1 ι2 Heq2. apply HQ.
@@ -401,24 +485,35 @@ Module Pred.
       Qed.
 
       Lemma wlp_true {w0 w1} (r01 : R w0 w1) :
-        wlp r01 PTrue ⊣⊢ PTrue.
+        wlp r01 Trueₚ ⊣⊢ₚ Trueₚ.
       Proof. firstorder. Qed.
 
       Lemma wlp_impl {w0 w1} (r01 : R w0 w1) P Q :
-        Entails (wlp r01 (P ⇒ Q)) (wlp r01 P ⇒ wlp r01 Q)%P.
+        wlp r01 (P ->ₚ Q) ⊢ₚ wlp r01 P ->ₚ wlp r01 Q.
       Proof. intros ι0. cbn. intros HPQ HP ι1 <-. firstorder. Qed.
 
       Lemma entails_wlp {w0 w1} (r01 : R w0 w1) P Q :
-        Entails (Ext P r01) Q -> Entails P (wlp r01 Q).
-      Proof. intros HPQ ι0 HP ι1 <-. revert HP. apply HPQ. Qed.
+        (Ext P r01 ⊢ₚ Q) <-> (P ⊢ₚ wlp r01 Q).
+      Proof.
+        cbv [entails Ext wlp].
+        split.
+        - intros HPQ ι0 HP ι1 <-. revert HP. apply HPQ.
+        - intros HPQ ι1 HP. now apply (HPQ (inst r01 ι1)).
+      Qed.
 
-      Lemma pvalid_wlp {w0 w1} (r01 : R w0 w1) Q :
-        PValid Q -> PValid (wlp r01 Q).
-      Proof. unfold PValid; cbn. firstorder. Qed.
+      Lemma entails_wp {w0 w1} (r01 : R w0 w1) P Q :
+        (P ⊢ₚ Ext Q r01) <-> (wp r01 P ⊢ₚ Q).
+      Proof.
+        cbv [entails Ext wp].
+        split.
+        - intros HPQ ι0 (ι1 & <- & HP). now apply HPQ.
+        - intros HPQ ι1 HP. apply (HPQ (inst r01 ι1)).
+          exists ι1. split; auto.
+      Qed.
 
       Lemma wlp_thick {thickR : Thick R} {instThickR : InstThick R}
-        {w x} (xIn : ctx.In x w) (t : Ty (ctx.remove xIn)) (Q : Pred (ctx.remove xIn))  :
-        wlp (thick x t) Q ⊣⊢ PEq (Ty_hole xIn) (thin xIn t) ⇒ Ext Q (Sub.thin xIn).
+        {w x} (xIn : ctx.In x w) (t : Ty (ctx.remove xIn)) (Q : Pred (ctx.remove xIn)) :
+        wlp (thick x t) Q ⊣⊢ₚ Ty_hole xIn =ₚ thin xIn t ->ₚ Ext Q (Sub.thin xIn).
       Proof.
         intros ι; cbn. rewrite Sub.subst_thin, inst_persist_ty, Sub.inst_thin.
         split; intros HQ.
@@ -429,125 +524,91 @@ Module Pred.
           now apply HQ.
       Qed.
 
+      Lemma wlp_step {stepR : Step R} {w} {x} (Q : Pred (ctx.snoc w x)):
+        wlp (w0:=w) step Q ⊣⊢ₚ (∀ₚ t ∶ Ty, Ext Q (thick (xIn := ctx.in_zero) x t)).
+      Proof.
+        intros ι. cbn - [thick]. unfold Forall.
+        split.
+        - intros HQ t. apply HQ.
+          rewrite (inst_thick ctx.in_zero t ι). cbn.
+          now rewrite inst_step_snoc.
+        - cbn - [thick]. intros HQ ι' <-.
+          destruct (env.view ι') as [ι t].
+          specialize (HQ (lift t _)).
+          rewrite inst_step_snoc in HQ.
+          rewrite (inst_thick ctx.in_zero (lift t w) ι) in HQ.
+          now rewrite inst_lift in HQ.
+      Qed.
+
     End WithAccessibilityRelation.
     (* #[global] Opaque wp. *)
     (* #[global] Opaque wlp. *)
   End Acc.
 
-  Lemma pno_cycle {w x} (xIn : ctx.In x w) (t : Ty w) :
-    Ty_subterm (Ty_hole xIn) t ->
-    Entails (Ty_hole xIn = t) PFalse.
+  Lemma pno_cycle {w} (t1 t2 : Ty w) :
+    Ty_subterm t1 t2 ->
+    t1 =ₚ t2  ⊢ₚ  ⊥ₚ.
   Proof.
     intros Hsub ι Heq.
     apply (inst_subterm ι) in Hsub. cbn in Hsub.
     rewrite <- Heq in Hsub. now apply ty_no_cycle in Hsub.
   Qed.
 
-  #[local] Notation Expr := (Sem expr).
-
-  Definition TPB : ⊢ Env -> Const expr -> Ty -> Expr -> Pred :=
-    fun w G e t ee ι => inst G ι |-- e ; inst t ι ~> inst ee ι.
-  #[global] Arguments TPB [w] G e t ee ι/.
-
-  (* #[global] Opaque BiEntails Entails PAnd PImpl PEq. *)
-
-  Module Import notations.
-
-    Notation "t1 ≃ t2" :=
-      (PEq t1 t2) (at level 90) : pred_scope.
-    Notation "'Fun' x => b" :=
-      (fun w ζ x => b%P w ζ)
-        (x binder, at level 100) : pred_scope.
-    Notation "⊩ P" := (PValid P) (at level 95).
-    Notation "P ⊣⊢ Q" := (BiEntails P Q) (at level 95).
-    Notation "⊤" := PTrue : pred_scope.
-    Notation "⊥" := PFalse : pred_scope.
-    Notation "P ⇔ Q" := (PIff P Q) (at level 94) : pred_scope.
-    Notation "P ⇒ Q" := (PImpl P Q) (at level 94, right associativity) : pred_scope.
-    Notation "P ∧ Q" := (PAnd P Q) (at level 80, right associativity) : pred_scope.
-
-    Notation "'∀' x ∶ T , Q" :=
-      (@Forall T _ (fun x => Q%P))
-        (at level 99, x binder, x at next level, T at level 95,
-          right associativity,
-          format "'∀'  x  ∶  T ,  Q")
-      : pred_scope.
-
-    Notation "'∀⁺' x .. y , Q " :=
-      (Forall (fun x => .. (Forall (fun y => Q%P)) ..))
-        (at level 99, x binder, y binder, right associativity,
-        only parsing)
-      : pred_scope.
-
-    (* Notation "'∃' x .. y , Q " := *)
-    (*     (Exists (fun x => .. (Exists (fun y => Q%P)) ..)) *)
-    (*       (at level 94, x binder, y binder, right associativity) *)
-    (*     : pred_scope. *)
-
-    Notation "'∃' x ∶ T , Q" :=
-      (@Exists T _ (fun x => Q%P))
-        (at level 99, x binder, right associativity,
-          format "'∃'  x  ∶  T ,  Q")
-        : pred_scope.
-
-    Notation "G |-- E ; T ~> EE" := (TPB G E T EE) : pred_scope.
-
-  End notations.
-
   (* A predicate-based induction scheme for the typing relation. *)
   Section InductionScheme.
 
     Context (P : ⊢ Env -> Const expr -> Ty -> Expr -> Pred).
     Context
-      {pfalse : forall w, PValid (w := w)
-         (∀ G ∶ Env, ∀ t ∶ Ty, ∀ e' ∶ Expr,
-             PEq t Ty_bool ⇒
-             PEq e' (S.pure v_false) ⇒
+      {pfalse : forall w,
+          entails (w := w) Trueₚ
+         (∀ₚ G ∶ Env, ∀ₚ t ∶ Ty, ∀ₚ e' ∶ Expr,
+             t =ₚ Ty_bool ->ₚ
+             e' =ₚ (S.pure v_false) ->ₚ
              P G v_false t e')%P }
-      {ptrue : forall w, PValid (w := w)
-         (∀ G ∶ Env, ∀ t ∶ Ty, ∀ e' ∶ Expr,
-             PEq t Ty_bool ⇒
-             PEq e' (S.pure v_true) ⇒
+      {ptrue : forall w, entails Trueₚ (w := w)
+         (∀ₚ G ∶ Env, ∀ₚ t ∶ Ty, ∀ₚ e' ∶ Expr,
+             t =ₚ Ty_bool ->ₚ
+             e' =ₚ (S.pure v_true) ->ₚ
              P G v_true t e')%P }
-      {pif : forall w, PValid (w := w)
-         (∀⁺ G e1 e2 e3 e' e1' e2' e3' t,
-             (G |-- e1; Ty_bool ~> e1') ⇒
-             (G |-- e2; t ~> e2') ⇒
-             (G |-- e3; t ~> e3') ⇒
-             P G e1 Ty_bool e1' ⇒
-             P G e2 t e2' ⇒
-             P G e3 t e3' ⇒
-             PEq e' (fun ι0 => e_if (e1' ι0) (e2' ι0) (e3' ι0)) ⇒
+      {pif : forall w, entails Trueₚ (w := w)
+         (∀ₚ⁺ G e1 e2 e3 e' e1' e2' e3' t,
+             (G |--ₚ e1; Ty_bool ~> e1') ->ₚ
+             (G |--ₚ e2; t ~> e2') ->ₚ
+             (G |--ₚ e3; t ~> e3') ->ₚ
+             P G e1 Ty_bool e1' ->ₚ
+             P G e2 t e2' ->ₚ
+             P G e3 t e3' ->ₚ
+             e' =ₚ (fun ι0 => e_if (e1' ι0) (e2' ι0) (e3' ι0)) ->ₚ
              P G (e_if e1 e2 e3) t e')%P }
-      {pvar : forall w (G : Env w) x t e', PValid
-         (PEq (resolve x G) (Some t) ⇒
-          PEq e' (fun _ => e_var x) ⇒
+      {pvar : forall w (G : Env w) x t e', entails Trueₚ
+         ((resolve x G) =ₚ (Some t) ->ₚ
+          e' =ₚ (fun _ => e_var x) ->ₚ
           P G (e_var x) t e') }
       {pabsu : forall w (G : Env w) x t1 t2 t e1 e1' e',
-        PValid
-          ((cons (x, t1) G |-- e1; t2 ~> e1') ⇒
-           P (cons (x, t1) G) e1 t2 e1' ⇒
-           PEq t (Ty_func t1 t2) ⇒
-           PEq e' (fun ι0 => e_abst x (inst t1 ι0) (e1' ι0)) ⇒
+        entails Trueₚ
+          ((cons (x, t1) G |--ₚ e1; t2 ~> e1') ->ₚ
+           P (cons (x, t1) G) e1 t2 e1' ->ₚ
+           t =ₚ (Ty_func t1 t2) ->ₚ
+           e' =ₚ (fun ι0 => e_abst x (inst t1 ι0) (e1' ι0)) ->ₚ
            P G (e_absu x e1) t e' )}
       {pabst : forall w (G : Env w) x t1 t2 e1 e1' e' t,
-          PValid
-            ((cons (x, lift t1 w) G |-- e1; t2 ~> e1') ⇒
-             P (cons (x, lift t1 w) G) e1 t2 e1' ⇒
-             PEq t (Ty_func (lift t1 w) t2) ⇒
-             PEq e' (fun ι0 => e_abst x t1 (e1' ι0)) ⇒
+          entails Trueₚ
+            ((cons (x, lift t1 w) G |--ₚ e1; t2 ~> e1') ->ₚ
+             P (cons (x, lift t1 w) G) e1 t2 e1' ->ₚ
+             t =ₚ (Ty_func (lift t1 w) t2) ->ₚ
+             e' =ₚ (fun ι0 => e_abst x t1 (e1' ι0)) ->ₚ
              P G (e_abst x t1 e1) t e')}
       {papp : forall w (G : Env w) e1 t1 e1' e2 t2 e2' e',
-          PValid
-            ((G |-- e1; Ty_func t2 t1 ~> e1') ⇒
-             (G |-- e2; t2 ~> e2') ⇒
-             P G e1 (Ty_func t2 t1) e1' ⇒
-             P G e2 t2 e2' ⇒
-             PEq e' (fun ι0 => e_app (e1' ι0) (e2' ι0)) ⇒
+          entails Trueₚ
+            ((G |--ₚ e1; Ty_func t2 t1 ~> e1') ->ₚ
+             (G |--ₚ e2; t2 ~> e2') ->ₚ
+             P G e1 (Ty_func t2 t1) e1' ->ₚ
+             P G e2 t2 e2' ->ₚ
+             e' =ₚ (fun ι0 => e_app (e1' ι0) (e2' ι0)) ->ₚ
              P G (e_app e1 e2) t1 e')%P }.
 
     Lemma TPB_ind w G (e : expr) (t : Ty w) (ee : Expr w) :
-      Entails (G |-- e; t ~> ee)%P (P G e t ee).
+      (G |--ₚ e; t ~> ee) ⊢ₚ (P G e t ee).
     Proof.
       intros ι T. hnf in T.
       remember (inst G ι) as G'.
@@ -581,6 +642,12 @@ Module Pred.
     Qed.
 
   End InductionScheme.
+
+  Definition ProperPost {R} {reflR : Refl R} {instR : forall w : World, Inst (R w) (Assignment w)}
+    {AT A} {persA : Persistent R AT} {instT : Inst AT A}
+    {w} (Q : Box R (AT -> Pred) w) : Prop :=
+    forall {w1} (r01 : R w w1) (te0 : AT w) (te1 : AT w1),
+      (te1 =ₚ (persist _ te0 _ r01)) ⊢ₚ (Ext (Q w refl te0) r01 <->ₚ Q w1 r01 te1).
 
 End Pred.
 Export Pred (Pred).
