theories/unification/CorrectnessWithAssignments.v
@@ -78,7 +78,7 @@ Module ProgramLogic.
     fun w0 d Q =>
       match d with
       | Some (w1; (r01, a)) => Acc.wp r01 (Q w1 r01 a)
-      | None                => PFalse
+      | None                => Falseₚ
       end.
 
   #[global] Arguments WP {A}%indexed_scope [w] _ _%P _.
@@ -89,7 +89,7 @@ Module ProgramLogic.
       (pointwise_relation _
          (forall_relation
             (fun _ => pointwise_relation _
-                        (pointwise_relation _ BiEntails)) ==> BiEntails))
+                        (pointwise_relation _ bientails)) ==> bientails))
       (@WP A w).
   Proof.
     intros d p q pq. destruct d as [(w1 & r01 & a)|]; cbn; [|easy].
@@ -101,7 +101,7 @@ Module ProgramLogic.
       (pointwise_relation _
          (forall_relation
             (fun _ => pointwise_relation _
-                        (pointwise_relation _ Entails)) ==> Entails))
+                        (pointwise_relation _ entails)) ==> entails))
       (@WP A w).
   Proof.
     intros d p q pq. destruct d as [(w1 & r01 & a)|]; cbn; [|easy].
@@ -110,26 +110,26 @@ Module ProgramLogic.
 
   Lemma wp_monotonic' {A w} (d : ◆A w) (R : Pred w) (P Q : □(A -> Pred) w) :
     (forall w1 (r : w ⊒⁻ w1) (a : A w1),
-        Entails (Ext R r) (P w1 r a ⇒ Q w1 r a)%P) ->
-    Entails R (WP d P ⇒ WP d Q)%P.
+        Ext R r ⊢ₚ P w1 r a ->ₚ Q w1 r a) ->
+    R ⊢ₚ WP d P ->ₚ WP d Q.
   Proof.
     intros pq. destruct d as [(w1 & r01 & a)|]; cbn.
     - specialize (pq w1 r01 a).
-      apply pimpl_and_adjoint.
+      apply impl_and_adjoint.
       rewrite Acc.and_wp_r.
       apply Acc.proper_wp_entails.
-      apply pimpl_and_adjoint.
+      apply impl_and_adjoint.
       apply pq.
-    - apply pimpl_and_adjoint.
-      now rewrite pand_false_r.
+    - apply impl_and_adjoint.
+      now rewrite and_false_r.
   Qed.
 
   Lemma wp_pure {A w0} (a : A w0) (Q : □(A -> Pred) w0) :
-    WP (η a) Q ⊣⊢ T Q a.
-  Proof. unfold WP, η. now rewrite Acc.wp_refl. Qed.
+    WP (pure a) Q ⊣⊢ₚ T Q a.
+  Proof. unfold WP, pure. cbn. now rewrite Acc.wp_refl. Qed.
 
   Lemma wp_bind {A B w0} (d : ◆A w0) (f : □(A -> ◆B) w0) (Q : □(B -> Pred) w0) :
-    WP (bind d f) Q ⊣⊢ WP d (fun w1 ζ1 a1 => WP (f w1 ζ1 a1) (_4 Q ζ1)).
+    WP (bind d f) Q ⊣⊢ₚ WP d (fun w1 ζ1 a1 => WP (f w1 ζ1 a1) (_4 Q ζ1)).
   Proof.
     destruct d as [(w1 & r01 & a)|]; cbn; [|reflexivity].
     destruct (f w1 r01 a) as [(w2 & r12 & b2)|]; cbn;
@@ -140,7 +140,7 @@ Module ProgramLogic.
     fun w0 d Q =>
       match d with
       | Some (w1; (r01, a)) => Pred.Acc.wlp r01 (Q w1 r01 a)
-      | None                => PTrue
+      | None                => Trueₚ
       end.
   #[global] Arguments WLP {A}%indexed_scope [w] _ _%P _.
   #[global] Instance params_wlp : Params (@WLP) 4 := {}.
@@ -150,7 +150,7 @@ Module ProgramLogic.
       (pointwise_relation _
          (forall_relation
             (fun _ => pointwise_relation _
-                        (pointwise_relation _ BiEntails)) ==> BiEntails))
+                        (pointwise_relation _ bientails)) ==> bientails))
       (@WLP A w).
   Proof.
     intros d p q pq. destruct d as [(w1 & r01 & a)|]; cbn; [|easy].
@@ -162,7 +162,7 @@ Module ProgramLogic.
       (pointwise_relation _
          (forall_relation
             (fun _ => pointwise_relation _
-                        (pointwise_relation _ Entails)) ==> Entails))
+                        (pointwise_relation _ entails)) ==> entails))
       (@WLP A w).
   Proof.
     intros d p q pq. destruct d as [(w1 & r01 & a)|]; cbn; [|easy].
@@ -171,21 +171,21 @@ Module ProgramLogic.
 
   Lemma wlp_monotonic' {A w} (d : ◆A w) (R : Pred w) (P Q : □(A -> Pred) w) :
     (forall w1 (r : w ⊒⁻ w1) (a : A w1),
-        Entails (Ext R r) (P w1 r a ⇒ Q w1 r a)%P) ->
-    Entails R (WLP d P ⇒ WLP d Q)%P.
+        entails (Ext R r) (P w1 r a ->ₚ Q w1 r a)%P) ->
+    entails R (WLP d P ->ₚ WLP d Q)%P.
   Proof.
     intros pq. destruct d as [(w1 & r01 & a)|]; cbn.
     - specialize (pq w1 r01 a). rewrite <- Acc.wlp_impl.
       now apply Acc.entails_wlp.
-    - rewrite pimpl_true_r. apply entails_true.
+    - rewrite impl_true_r. apply true_r.
   Qed.
 
   Lemma wlp_pure {A w} (a : A w) (Q : □(A -> Pred) w) :
-    WLP (η a) Q ⊣⊢ T Q a.
-  Proof. unfold WLP, η. now rewrite Acc.wlp_refl. Qed.
+    WLP (pure a) Q ⊣⊢ₚ T Q a.
+  Proof. unfold WLP, pure. cbn. now rewrite Acc.wlp_refl. Qed.
 
   Lemma wlp_bind {A B w0} (d : ◆A w0) (f : □(A -> ◆B) w0) (Q : □(B -> Pred) w0) :
-    WLP (bind d f) Q ⊣⊢ WLP d (fun w1 ζ1 a1 => WLP (f w1 ζ1 a1) (_4 Q ζ1)).
+    WLP (bind d f) Q ⊣⊢ₚ WLP d (fun w1 ζ1 a1 => WLP (f w1 ζ1 a1) (_4 Q ζ1)).
   Proof.
     destruct d as [(w1 & r01 & a)|]; cbn; [|reflexivity].
     destruct (f w1 r01 a) as [(w2 & r12 & b2)|]; cbn;
@@ -193,35 +193,102 @@ Module ProgramLogic.
   Qed.
 
   Lemma wlp_tell1 {w x} (xIn : x ∈ w) (t : Ty (w - x)) (Q : □(Unit -> Pred) w) :
-    WLP (tell1 xIn t) Q ⊣⊢ Acc.wlp (thick x t) (Q _ (thick x t) tt).
+    WLP (tell1 xIn t) Q ⊣⊢ₚ Acc.wlp (thick x t) (Q _ (thick x t) tt).
   Proof. reflexivity. Qed.
 
 End ProgramLogic.
 
 Module Correctness.
 
-  Import (hints) Tri.
+  Import (hints) Pred.Acc Tri.
   Import Pred Pred.notations ProgramLogic.
+
+  Definition interpM : ⊢ M Unit -> Pred :=
+    fun w m => WP m (fun _ _ _ => Trueₚ).
+
+  Definition interpC : ⊢ C -> Pred.
+  Proof.
+    intros w m.
+    unfold C in m.
+    refine (WP (m w refl) (fun _ _ _ => Trueₚ)).
+  Defined.
+
+  (* Lemma ctrue_correct {w : World} : BiEntails (w := w) (interp ctrue) PTrue. *)
+  (* Proof. unfold interp, ctrue. now rewrite wp_pure. Qed. *)
+
+  (* Lemma cfalse_correct {w : World} : BiEntails (w := w) (interp cfalse) PFalse. *)
+  (* Proof. unfold interp, cfalse. easy. Qed. *)
+
+  Opaque bind.
+  Import LR.
+
+  Definition ProperRC {w} (c : C w) : Prop :=
+    forall w' (r : Tri w w'),
+      Acc.wp r (WP (c w' r) (fun _ _ _ => Trueₚ)) ⊣⊢ₚ
+      Acc.wp r Trueₚ /\ₚ WP (c w refl) (fun _ _ _ => Trueₚ).
+
+  Lemma proper_ctrue {w0} : @ProperRC w0 ctrue.
+  Proof.
+    unfold ProperRC, ctrue; intros w1 r01. cbn.
+    now rewrite ?Acc.wp_refl, and_true_r.
+  Qed.
+
+  Lemma proper_cfalse {w0} : @ProperRC w0 cfalse.
+  Proof.
+    unfold ProperRC, cfalse; intros w1 r01. cbn.
+    now rewrite Acc.wp_false, and_false_r.
+  Qed.
+
+  Lemma proper_cand {w0} (c1 c2 : C w0) :
+    ProperRC c1 -> ProperRC c2 -> ProperRC (cand c1 c2).
+  Proof.
+    unfold ProperRC, cand; intros p1 p2 w1 r01.
+    unfold interpM in *. rewrite ?wp_bind. unfold _4.
+    specialize (p1 w1 r01).
+    destruct (c1 w0 refl) as [(w2 & r02 & [])|],
+        (c1 w1 r01)  as [(w3 & r13 & [])|];
+      cbn in *; rewrite ?Acc.wp_false, ?ext_false, ?pand_false_r in *.
+    - rewrite <- Acc.wp_trans in *. rewrite p2. rewrite p2. clear p2.
+      rewrite p1. unfold bientails, andₚ. intuition.
+    - rewrite p2. apply split_bientails. split.
+      + intros ? [].
+      + rewrite p1. unfold entails, andₚ. intuition.
+    - rewrite <- Acc.wp_trans in *.
+      now rewrite p2, p1, and_false_r, and_false_l.
+    - easy.
+  Qed.
+
+  Lemma cand_correct {w} {c1 c2 : C w} {p2 : ProperRC c2} :
+    interpC (cand c1 c2) ⊣⊢ₚ interpC c1 /\ₚ interpC c2.
+  Proof.
+    unfold interpC, cand. rewrite wp_bind.
+    destruct (c1 w refl) as [(w1 & r01 & [])|];
+      cbn; [|now rewrite and_false_l].
+    unfold _4.
+    rewrite Acc.and_wp_l, and_true_l, trans_refl_l.
+    rewrite (p2 w1 r01).
+    now rewrite Acc.and_wp_l, and_true_l.
+  Qed.
 
   Definition UnifierSound : ⊢ Unifier -> PROP :=
     fun w0 u =>
       forall (t1 t2 : Ty w0),
-        ⊩ WLP (u t1 t2) (Fun _ => Ext (t1 ≃ t2)).
+        ⊤ₚ ⊢ₚ WLP (u t1 t2) (Fun _ => Ext (t1 =ₚ t2)).
 
   Definition UnifierComplete : ⊢ Unifier -> PROP :=
     fun w0 u =>
       forall (t1 t2 : Ty w0),
-        ⊩ t1 ≃ t2 ⇒ WP (u t1 t2) (fun _ _ _ => PTrue).
+        t1 =ₚ t2 ⊢ₚ WP (u t1 t2) (fun _ _ _ => ⊤ₚ)%P.
 
   Definition BoxUnifierSound : ⊢ BoxUnifier -> PROP :=
     fun w0 bu =>
       forall (t1 t2 : Ty w0) (w1 : World) (ζ01 : w0 ⊒⁻ w1),
-        ⊩ WLP (bu t1 t2 w1 ζ01) (Fun _ => Ext (Ext (t1 ≃ t2) ζ01)).
+        ⊤ₚ ⊢ₚ WLP (bu t1 t2 w1 ζ01) (Fun _ => Ext (Ext (t1 =ₚ t2) ζ01)).
 
   Definition BoxUnifierComplete : ⊢ BoxUnifier -> PROP :=
     fun w0 bu =>
       forall (t1 t2 : Ty w0) (w1 : World) (ζ01 : w0 ⊒⁻ w1),
-        Entails (Ext (t1 ≃ t2) ζ01) (WP (bu t1 t2 w1 ζ01) (fun _ _ _ => PTrue)).
+        entails (Ext (t1 =ₚ t2) ζ01) (WP (bu t1 t2 w1 ζ01) (fun _ _ _ => Trueₚ)).
 
   Section BoxedProofs.
 
@@ -234,38 +301,66 @@ Module Correctness.
                   BoxUnifierSound (lmgu xIn)).
 
       Lemma flex_sound_assignment {x} (xIn : x ∈ w) (t : Ty w) :
-        ⊩ WLP (flex t xIn) (Fun _ => Ext (Ty_hole xIn ≃ t)).
+        ⊤ₚ ⊢ₚ WLP (flex t xIn) (Fun _ => Ext (Ty_hole xIn =ₚ t)).
       Proof.
         unfold flex. destruct (varview t) as [y yIn|].
         - destruct (ctx.occurs_check_view xIn yIn).
-          + rewrite wlp_pure. unfold T. now rewrite ext_refl.
-          + rewrite wlp_tell1. apply Acc.pvalid_wlp.
-            rewrite <- peq_persist. cbn. unfold thickIn.
+          + rewrite wlp_pure. unfold T.
+            rewrite ext_refl, eqₚ_refl.
+            reflexivity.
+          + rewrite wlp_tell1. rewrite <- Acc.entails_wlp.
+            rewrite ext_true, ext_eq. cbn. unfold thickIn.
             rewrite ctx.occurs_check_view_refl, ctx.occurs_check_view_thin.
-            easy.
+            rewrite eqₚ_refl. reflexivity.
         - destruct (occurs_check_spec xIn t); subst; [|constructor].
-          rewrite wlp_tell1, <- peq_persist, persist_thin_thick.
-          apply Acc.pvalid_wlp. cbn. unfold thickIn.
-          rewrite ctx.occurs_check_view_refl. easy.
+          rewrite wlp_tell1, ext_eq, persist_thin_thick.
+          rewrite <- Acc.entails_wlp, ext_true. cbn. unfold thickIn.
+          rewrite ctx.occurs_check_view_refl. rewrite eqₚ_refl. reflexivity.
       Qed.
 
       Lemma boxflex_sound_assignment {x} (xIn : x ∈ w) (t : Ty w)
         {w1} (ζ01 : w ⊒⁻ w1) :
-        ⊩ WLP (boxflex lmgu t xIn ζ01) (Fun _ => Ext (Ext (Ty_hole xIn ≃ t) ζ01)).
+        ⊤ₚ ⊢ₚ WLP (boxflex lmgu t xIn ζ01) (Fun _ => Ext (Ext (Ty_hole xIn =ₚ t) ζ01)).
       Proof.
         unfold boxflex, Tri.box_intro_split.
         destruct ζ01 as [|w2 y yIn ty]; folddefs.
         - generalize (flex_sound_assignment xIn t).
-          apply proper_pvalid_entails.
+          apply proper_entails_entails; [easy|].
           apply proper_wlp_entails.
           intros w2 ζ2 _.
           now rewrite ext_refl.
         - generalize (lmgu_sound yIn (Ty_hole xIn)[thick y ty] t[thick y ty] ζ01). clear.
-          apply proper_pvalid_entails.
+          apply proper_entails_entails; [easy|].
           apply proper_wlp_entails.
           intros w3 ζ3 _.
-          now rewrite ext_trans, peq_persist.
+          now rewrite ext_trans, ?ext_eq.
       Qed.
+
+      Lemma wp_ctrue {w0 w1} (r01 : w0 ⊒⁻ w1) (Q : □(Unit -> Pred) w1) :
+        WP (ctrue r01) Q ⊣⊢ₚ T Q tt.
+      Proof. unfold ctrue. now rewrite wp_pure. Qed.
+
+      Lemma wp_cfalse {w0 w1} (r01 : w0 ⊒⁻ w1) (Q : □(Unit -> Pred) w1) :
+        WP (cfalse r01) Q ⊣⊢ₚ Falseₚ.
+      Proof. reflexivity. Qed.
+
+      Lemma wp_cand {w0 w1} (r01 : w0 ⊒⁻ w1) m1 m2 (Q : □(Unit -> Pred) w1) :
+        WP (cand m1 m2 r01) Q ⊣⊢ₚ
+        WP (m1 w1 r01) (fun w2 r12 _ => WP (_4 m2 r01 r12) (_4 Q r12)).
+      Proof. unfold cand. now rewrite wp_bind. Qed.
+
+      Lemma wlp_ctrue {w0 w1} (r01 : w0 ⊒⁻ w1) (Q : □(Unit -> Pred) w1) :
+        WLP (ctrue r01) Q ⊣⊢ₚ T Q tt.
+      Proof. unfold ctrue. now rewrite wlp_pure. Qed.
+
+      Lemma wlp_cfalse {w0 w1} (r01 : w0 ⊒⁻ w1) (Q : □(Unit -> Pred) w1) :
+        WLP (cfalse r01) Q ⊣⊢ₚ Trueₚ.
+      Proof. reflexivity. Qed.
+
+      Lemma wlp_cand {w0 w1} (r01 : w0 ⊒⁻ w1) m1 m2 (Q : □(Unit -> Pred) w1) :
+        WLP (cand m1 m2 r01) Q ⊣⊢ₚ
+        WLP (m1 w1 r01) (fun w2 r12 _ => WLP (_4 m2 r01 r12) (_4 Q r12)).
+      Proof. unfold cand. now rewrite wlp_bind. Qed.
 
       Lemma boxmgu_sound_assignment : BoxUnifierSound (boxmgu lmgu).
       Proof.
@@ -273,23 +368,27 @@ Module Correctness.
         apply boxmgu_elim; clear t1 t2.
         - intros. apply boxflex_sound_assignment.
         - intros. generalize (boxflex_sound_assignment xIn t ζ01).
-          apply proper_pvalid_entails, proper_wlp_entails.
-          intros w2 r12 _. now rewrite peq_symmetry.
-        - intros *. now rewrite wlp_pure.
-        - constructor.
-        - constructor.
-        - intros * IH1 IH2 *. rewrite wlp_bind.
+          apply proper_entails_entails; [easy|].
+          apply proper_wlp_entails.
+          intros w2 r12 _. now rewrite eqₚ_symmetry.
+        - intros *. now rewrite wlp_ctrue.
+        - intros *. now rewrite wlp_cfalse.
+        - intros *. now rewrite wlp_cfalse.
+        - intros * IH1 IH2 *. rewrite wlp_cand.
           specialize (IH1 _ ζ01). revert IH1.
-          apply proper_pvalid_entails, proper_wlp_entails.
-          intros w2 ζ12 _. rewrite wlp_bind.
-          apply (pGeneralize (IH2 _ (ζ01 ⊙ ζ12))), wlp_monotonic'.
-          intros ? ? _. rewrite wlp_pure. unfold T, _4.
-          rewrite ?trans_refl_r, ?ext_trans, ?ext_impl.
+          apply proper_entails_entails; [easy|].
+          apply proper_wlp_entails.
+          intros w2 ζ12 _. unfold _4.
+          specialize (IH2 _ (ζ01 ⊙ ζ12)).
+          rewrite <- and_true_r, IH2. apply impl_and_adjoint.
+          apply wlp_monotonic'.
+          intros ? ? _.
+          rewrite ?trans_refl_r, ?ext_trans, <- ?ext_impl.
           apply proper_ext_entails; auto.
           apply proper_ext_entails; auto.
           apply proper_ext_entails; auto.
           rewrite (peq_ty_noconfusion (Ty_func s1 s2)).
-          now apply pimpl_and_adjoint.
+          now apply impl_and_adjoint.
       Qed.
 
     End Soundness.
@@ -299,30 +398,27 @@ Module Correctness.
                   BoxUnifierComplete (lmgu xIn)).
 
       Lemma flex_complete_assignment {x} (xIn : x ∈ w) (t : Ty w) :
-        Entails
-          (Ty_hole xIn ≃ t)%P
-          (WP (flex t xIn) (fun (w0 : World) (_ : w ⊒⁻ w0) (_ : Unit w0) => ⊤%P)).
+        Ty_hole xIn =ₚ t ⊢ₚ WP (flex t xIn) (fun _ _ _ => ⊤ₚ)%P.
       Proof.
         unfold flex. destruct (varview t) as [y yIn|].
         - destruct (ctx.occurs_check_view xIn yIn).
-          + rewrite wp_pure. unfold T. apply entails_true.
-          + unfold WP, tell1. now rewrite Acc.wp_thick, ext_true, pand_true_r.
+          + rewrite wp_pure. unfold T. apply true_r.
+          + unfold WP, tell1. now rewrite Acc.wp_thick, ext_true, and_true_r.
         - destruct (occurs_check_spec xIn t) as [|[HOC|HOC]]; cbn.
-          + subst. now rewrite Acc.wp_thick, ext_true, pand_true_r.
+          + subst. now rewrite Acc.wp_thick, ext_true, and_true_r.
           + destruct (H _ _ HOC).
           + now apply pno_cycle in HOC.
       Qed.
 
       Lemma boxflex_complete_assignment {x} (xIn : x ∈ w) (t : Ty w) {w1} (ζ01 : w ⊒⁻ w1) :
-        Entails
-          (Ext (Ty_hole xIn ≃ t) ζ01)
-          (WP (boxflex lmgu t xIn ζ01) (fun (w0 : World) (_ : w1 ⊒⁻ w0) (_ : Unit w0) => ⊤%P)).
+        Ext (Ty_hole xIn =ₚ t) ζ01 ⊢ₚ
+        WP (boxflex lmgu t xIn ζ01) (fun _ _ _ => ⊤ₚ)%P.
       Proof.
         unfold boxflex, Tri.box_intro_split.
         destruct ζ01 as [|w2 y yIn ty]; folddefs.
         - rewrite ext_refl. apply flex_complete_assignment.
         - change (Tri.cons ?x ?t ?r) with (thick x t ⊙ r).
-          rewrite ext_trans, <- peq_persist.
+          rewrite ext_trans, ext_eq.
           now apply (lmgu_complete yIn).
       Qed.
 
@@ -331,26 +427,23 @@ Module Correctness.
         intros t1 t2. pattern (boxmgu lmgu t1 t2).
         apply boxmgu_elim; clear t1 t2.
         - intros. apply boxflex_complete_assignment.
-        - intros. rewrite peq_symmetry. apply boxflex_complete_assignment.
-        - intros *. rewrite wp_pure. apply entails_true.
+        - intros. rewrite eqₚ_symmetry. apply boxflex_complete_assignment.
+        - intros *. rewrite wp_ctrue. apply true_r.
         - intros. now rewrite peq_ty_noconfusion, ext_false.
         - intros. now rewrite peq_ty_noconfusion, ext_false.
         - intros * IH1 IH2 *.
-          rewrite wp_bind, peq_ty_noconfusion.
-          rewrite <- ext_and.
-          apply pimpl_and_adjoint.
+          rewrite wp_cand, peq_ty_noconfusion.
+          rewrite ext_and.
+          apply impl_and_adjoint.
           apply (pApply (IH1 w1 ζ01)). clear IH1.
-          apply pimpl_and_adjoint.
-          rewrite pand_comm.
-          apply pimpl_and_adjoint.
+          apply impl_and_adjoint.
+          rewrite and_comm.
+          apply impl_and_adjoint.
           apply wp_monotonic'. intros.
-          rewrite pimpl_true_l.
-          rewrite wp_bind.
+          rewrite impl_true_l. unfold _4.
           rewrite <- ext_trans.
           apply (pApply (IH2 _ _)).
-          apply proper_wp_entails. intros ? ? _.
-          rewrite wp_pure. unfold _4, T.
-          reflexivity.
+          now apply proper_wp_entails.
       Qed.
 
     End Completeness.
@@ -372,63 +465,67 @@ Module Correctness.
   Definition mgu_sound w : UnifierSound (@mgu w).
   Proof.
     unfold UnifierSound, mgu. intros t1 t2.
-    generalize (bmgu_sound t1 t2 refl).
-    apply proper_pvalid_entails, proper_wlp_entails.
+    specialize (bmgu_sound t1 t2 refl).
+    apply proper_entails_entails; [easy|].
+    apply proper_wlp_entails.
     intros w' r _. now rewrite ext_refl.
   Qed.
 
   Definition mgu_complete w : UnifierComplete (@mgu w).
   Proof.
-    unfold UnifierComplete, mgu. intros t1 t2. apply pIntro.
-    apply (pApply_r (@bmgu_complete _ t1 t2 _ refl)).
+    unfold UnifierComplete, mgu. intros t1 t2.
+    specialize (@bmgu_complete _ t1 t2 _ refl).
     now rewrite ext_refl.
   Qed.
 
   Import Pred.
 
   #[local] Instance instpred_prod_ty : InstPred (Prod Ty Ty) :=
-    fun w '(t1,t2) => PEq t1 t2.
+    fun w '(t1,t2) => eqₚ t1 t2.
 
   Definition BoxSolveListSound : ⊢ BoxSolveList -> PROP :=
     fun w0 bsl =>
       forall (C : List (Prod Ty Ty) w0) (w1 : World) (ζ01 : w0 ⊒⁻ w1),
-        ⊩ WLP (bsl C w1 ζ01) (Fun _ => Ext (Ext (instpred C) ζ01)).
+        ⊤ₚ ⊢ₚ WLP (bsl C w1 ζ01) (Fun _ => Ext (Ext (instpred C) ζ01)).
 
   Definition SolveListSound : ⊢ SolveList -> PROP :=
     fun w0 sl =>
       forall (C : List (Prod Ty Ty) w0),
-        ⊩ WLP (sl C) (Fun _ => Ext (instpred C)).
+        ⊤ₚ ⊢ₚ WLP (sl C) (Fun _ => Ext (instpred C)).
 
   Definition BoxSolveListComplete : ⊢ BoxSolveList -> PROP :=
     fun w0 bsl =>
       forall (C : List (Prod Ty Ty) w0) (w1 : World) (ζ01 : w0 ⊒⁻ w1),
-        Entails (Ext (instpred C) ζ01) (WP (bsl C w1 ζ01) (fun _ _ _ => PTrue)).
+        entails (Ext (instpred C) ζ01) (WP (bsl C w1 ζ01) (fun _ _ _ => Trueₚ)).
 
   Definition SolveListComplete : ⊢ SolveList -> PROP :=
     fun w0 sl =>
       forall (C : List (Prod Ty Ty) w0),
-        Entails (instpred C) (WP (sl C) (fun _ _ _ => PTrue)).
+        entails (instpred C) (WP (sl C) (fun _ _ _ => Trueₚ)).
 
   Lemma boxsolvelist_sound {w} : BoxSolveListSound (boxsolvelist (w := w)).
   Proof.
-    intros C. induction C as [|[t1 t2]]; cbn; intros.
-    - rewrite Acc.wlp_refl. easy.
-    - rewrite wlp_bind. generalize (bmgu_sound t1 t2 ζ01).
-      apply proper_pvalid_entails, proper_wlp_entails.
-      intros w2 r2 _. apply (pGeneralize (IHC _ (ζ01 ⊙⁻ r2))).
-      apply wlp_monotonic'. unfold _4. intros w3 r3 _.
-      rewrite ?trans_refl_r, ?ext_trans, ?ext_impl.
+    intros C. induction C as [|[t1 t2]]; cbn - [ctrue cand]; intros.
+    - now rewrite wlp_ctrue.
+    - rewrite wlp_cand. generalize (bmgu_sound t1 t2 ζ01).
+      apply proper_entails_entails; [easy|].
+      apply proper_wlp_entails. intros w2 r2 _.
+      rewrite <- and_true_r, (IHC _ (ζ01 ⊙⁻ r2)).
+      apply impl_and_adjoint, wlp_monotonic'.
+      unfold _4. intros w3 r3 _.
+      rewrite ?trans_refl_r, ?ext_trans, <- ?ext_impl.
       apply proper_ext_entails; auto.
       apply proper_ext_entails; auto.
       apply proper_ext_entails; auto.
-      now apply pimpl_and_adjoint.
+      now apply impl_and_adjoint.
   Qed.
 
   Lemma solvelist_sound {w} : SolveListSound (solvelist (w := w)).
   Proof.
     unfold SolveListSound, solvelist. intros C.
     generalize (boxsolvelist_sound C refl).
-    apply proper_pvalid_entails, proper_wlp_entails.
+    apply proper_entails_entails; [easy|].
+    apply proper_wlp_entails.
     intros w' r _. now rewrite ext_refl.
   Qed.
 
@@ -436,14 +533,11 @@ Module Correctness.
   Proof.
     intros C. induction C as [|[t1 t2]]; cbn; intros.
     - rewrite Acc.wp_refl. easy.
-    - rewrite wp_bind. rewrite <- ext_and.
-      apply pimpl_and_adjoint.
-      apply (pApply (@bmgu_complete _ t1 t2 _ ζ01)).
-      apply pimpl_and_adjoint.
-      rewrite pand_comm.
-      apply pimpl_and_adjoint.
+    - rewrite wp_cand. rewrite ext_and.
+      rewrite (@bmgu_complete _ t1 t2 _ ζ01).
+      rewrite and_comm. apply impl_and_adjoint.
       apply wp_monotonic'. intros.
-      rewrite pimpl_true_l, <- ext_trans.
+      rewrite impl_true_l, <- ext_trans.
       apply IHC.
   Qed.
 
@@ -457,38 +551,39 @@ Module Correctness.
   Definition wp_prenex {A} : ⊢ ?◇⁺(List (Ty * Ty) * A) -> □⁺(A -> Pred) -> Pred :=
     fun w o Q =>
       match o with
-      | Some (w'; (r, (C, a))) => Acc.wp r (instpred C ∧ Q _ r a)
-      | None => PFalse
+      | Some (w'; (r, (C, a))) => Acc.wp r (instpred C /\ₚ Q _ r a)
+      | None => Falseₚ
       end.
 
+  Arguments Acc.wp {R _ w0 w1} r01 Q _/.
+
   Lemma prenex_correct {A w} (m : FreeM A w) (Q : □⁺(A -> Pred) w) :
-    wp_prenex (prenex m) Q ⊣⊢ STLC.WP m Q.
+    wp_prenex (prenex m) Q ⊣⊢ₚ STLC.WP m Q.
   Proof.
     unfold wp_prenex.
     induction m; cbn.
-    - rewrite Acc.wp_refl. rewrite pand_true_l. reflexivity.
+    - rewrite Acc.wp_refl. rewrite and_true_l. reflexivity.
     - reflexivity.
     - destruct (prenex m) as [(w' & r & C & a)|]; cbn.
-      + change (Acc.wp r (((t[r] ≃ t0[r]) ∧ instpred C) ∧ Q w' r a)
-          ⊣⊢ PEq t t0 ∧ STLC.WP m Q).
+      + change (Acc.wp r (((t[r] =ₚ t0[r]) /\ₚ instpred C) /\ₚ Q w' r a)
+          ⊣⊢ₚ t =ₚ t0 /\ₚ STLC.WP m Q).
         rewrite <- IHm.
         rewrite Acc.and_wp_r.
         apply Acc.proper_wp_bientails.
-        rewrite <- peq_persist.
-        unfold BiEntails, PAnd.
-        intros ι; cbn; intuition.
-      + change (PFalse ⊣⊢ (PEq t t0 ∧ STLC.WP m Q)).
-        rewrite <- IHm. now rewrite pand_false_r.
-    - unfold BiEntails, PAnd, PEq, _4, Acc.wp in *.
-      intros ι. destruct (prenex m) as [(w' & r & C & a)|]; cbn.
-      + split.
-        * intros (ι' & Heq & HC & HQ). subst. cbn.
-          remember (inst r ι') as ι. destruct (env.view ι).
-          exists v. apply IHm. exists ι'. rewrite Heqι.
-          split. easy. split; auto.
-        * intros (t & Hwp). apply IHm in Hwp.
-          destruct Hwp as (ι' & Heq & HC & HQ).
-          exists ι'. cbn. rewrite Heq. cbn. auto.
+        now rewrite ext_eq, and_assoc.
+      + change (Falseₚ ⊣⊢ₚ (t =ₚ t0 /\ₚ STLC.WP m Q)).
+        rewrite <- IHm. now rewrite and_false_r.
+    - destruct (prenex m) as [(w' & r & C & a)|]; cbn.
+      + change (alloc.fresh _ ?x _ ?r) with (step ⊙ r).
+        assert
+          (Acc.wp (step ⊙ r) (instpred C /\ₚ Q w' (alloc.fresh Σ i w' r) a)
+             ⊣⊢ₚ Acc.wp step (STLC.WP m (_4 Q step)))
+          as -> by now rewrite Acc.wp_trans, <- IHm.
+        intros ι; cbn; split.
+        * intros (ι' & Heq & HQ). destruct env.view as [ι' t]. subst ι'.
+          now exists t.
+        * intros (t & Hwp). apply IHm in Hwp. exists (env.snoc ι _ t). cbn.
+          split. auto. now apply IHm.
       + split; [easy|]. intros (t & Hwp). now apply IHm in Hwp.
   Qed.
 
@@ -496,12 +591,15 @@ Module Correctness.
     fun w m Q =>
       match m with
       | Some (w1; (r01, a)) => Acc.wp r01 (Q w1 r01 a)
-      | None => PFalse
+      | None => Falseₚ
       end.
 
-  Lemma solvefree_equiv {A} {pA : Persistent Tri.Tri A}
-    (m : FreeM A ctx.nil) (Q : □⁺(A -> Pred) [ctx]) :
-    wp_optiondiamond (solvefree m) Q ⊣⊢ STLC.WP m Q.
+  Lemma solvefree_equiv {AT A} {instA : Inst AT A}
+    {persAllocA : Persistent Alloc AT}
+    {persTriA : Persistent Tri.Tri AT}
+    (m : FreeM AT ctx.nil) (Q : □⁺(AT -> Pred) [ctx])
+    (RQ : ProperPost Q) :
+    wp_optiondiamond (solvefree m) Q ⊣⊢ₚ STLC.WP m Q.
   Proof.
     rewrite <- prenex_correct. unfold solvefree.
     unfold wp_prenex, wp_optiondiamond.
@@ -511,13 +609,16 @@ Module Correctness.
     destruct solvelist as [(w2 & r2 & [])|]; cbn in *.
     - apply split_bientails. split.
       + intros ι0 (ι2 & Heq & HQ); subst. exists (inst r2 ι2).
-        specialize (Hsound (inst r2 ι2) ι2 eq_refl). hnf in Hsound.
-        unfold PAnd. repeat split.
+        specialize (Hsound (inst r2 ι2) I ι2 eq_refl). hnf in Hsound.
+        unfold andₚ. repeat split.
         * destruct (env.view (inst r1 (inst r2 ι2))).
           destruct (env.view (inst alloc.nil_l ι2)).
           reflexivity.
         * assumption.
-        * clear - HQ. admit.
+        * admit.
+          (* epose proof (RQ w1 r1 _ a (inst r2 ι2)) as H1. *)
+          (* epose proof (RQ w2 alloc.nil_l _ (persist _ a _ r2) ι2) as H2. *)
+          (* cbn in H1, H2. *)
       + intros ι0 (ι1 & Heq1 & HC & HQ).
         specialize (Hcompl ι1 HC). destruct Hcompl as (ι2 & Heq2 & _).
         exists ι2. split. subst.
@@ -538,31 +639,31 @@ Module Generalized.
 
   Lemma wp_tell {w x} (xIn : x ∈ w) (t : Ty (w - x)) (Q : □(Unit -> Pred) w)
     (RQ : RProper (RBox (RImpl RUnit (RPred Tri))) Q) :
-    WP (tell1 xIn t) Q ⊣⊢ (Ty_hole xIn ≃ thin xIn t) ∧ T Q tt.
+    WP (tell1 xIn t) Q ⊣⊢ₚ Ty_hole xIn =ₚ thin xIn t /\ₚ T Q tt.
   Proof.
     unfold WP, tell1. rewrite Acc.wp_thick. intros ι. cbn.
     rewrite Sub.subst_thin, inst_persist_ty, Sub.inst_thin.
     apply and_iff_compat_l'. intros Heq.
-    specialize (RQ ι w (w - x) refl (thick x t) (thick x t) (env.remove _ ι xIn)).
-    cbv [RProper PValid RBox Forall Const PImpl Acc.wlp PEq
-      RImpl RUnit PTrue RPred PIff Ext] in RQ.
+    specialize (RQ ι I w (w - x) refl (thick x t) (thick x t) (env.remove _ ι xIn)).
+    cbv [RProper RBox Forall Const implₚ Acc.wlp eqₚ
+      RImpl RUnit Trueₚ RPred iffₚ Ext] in RQ.
     cbn in RQ. rewrite <- Heq, env.insert_remove in RQ.
     now specialize (RQ eq_refl eq_refl tt tt I).
   Qed.
 
   Lemma flex_correct {w x} (xIn : x ∈ w) (t : Ty w)
     (Q : □(Unit -> Pred) w) (RQ : RProper (RBox (RImpl RUnit (RPred Tri))) Q) :
-    WP (flex t xIn) Q ⊣⊢ (Ty_hole xIn ≃ t) ∧ T Q tt.
+    WP (flex t xIn) Q ⊣⊢ₚ Ty_hole xIn =ₚ t /\ₚ T Q tt.
   Proof.
     unfold flex. destruct (varview t) as [y yIn|].
     - destruct (ctx.occurs_check_view xIn yIn).
-      + now rewrite wp_pure, peq_refl, pand_true_l.
+      + now rewrite wp_pure, eqₚ_refl, and_true_l.
       + now rewrite wp_tell.
     - destruct (occurs_check_spec xIn t) as [|[HOC|HOC]]; cbn - [tell1].
       + rewrite wp_tell; now subst.
       + destruct (H _ _ HOC).
-      + apply pno_cycle in HOC. apply split_bientails. split; [apply entails_false|].
-        now rewrite HOC, pand_false_l.
+      + apply pno_cycle in HOC. apply split_bientails. split; [apply false_l|].
+        now rewrite HOC, and_false_l.
   Qed.
 
 End Generalized.
